UtilLemmas.v
@@ -1,0 +1,22 @@
+Lemma not_none_is_some : forall {A : Type} (y : option A),
+  y <> None -> exists x, y = Some x.
+Proof.
+  intros A y H.
+  destruct y as [x|].
+  - exists x. reflexivity.
+  - exfalso. apply H. reflexivity.
+Qed.
+
+(* This is what I am going to call the Joe subtlety in honor of
+   https://gist.github.com/jtassarotti/57f65712869af462a01b46b660e0d92d 
+   This is the buggy lemma here:
+   Lemma some_is_not_none : forall {A : Type} (y : option A),
+       exists x, y = Some x -> y <> None.
+   Btw, as of Aug 4, 2025, Copilot points this out *)
+Lemma some_is_not_none : forall {A : Type} (y : option A) (x: A),
+  y = Some x -> y <> None.
+Proof.
+  intros A y x H.
+  rewrite H.
+  discriminate.
+Qed.
